fun_defs.v
@@ -51,13 +51,11 @@ Notation " 'CALL' f 'ON' x " := (fe_call  f x) (at level 25, f at level 0, forma
 
 Open Scope expr_scope.
 
-Definition fun_prog := env Fun (Var*fun_expr).
-
 Reserved Notation " f '//' s '~~>' v" (at level 70, no associativity).
 
 Section fun_sem.
 
-  Variable P : fun_prog.
+  Variable (param : Fun -> Var) (body : Fun -> fun_expr).
 
   Inductive fun_sem : fun_expr -> env Var bt -> bt -> Prop := 
     | in_fs_var  : forall x e,                       £ x // e ~~> e⇢x
@@ -74,9 +72,8 @@ Section fun_sem.
     | in_fs_let : forall x f g e a b,                  f // e ~~> a
                             ->                         g // e⦃x⇠a⦄ ~~> b
                             ->            LET x::=f IN g // e ~~> b
-    | in_fs_call : forall p x f g e a b,               P⇢p = (x,f)
-                            ->                         g // e ~~> a
-                            ->                         f // e⦃x⇠a⦄ ~~> b
+    | in_fs_call : forall p g e a b,                   g // e ~~> a
+                            ->                    body p // e⦃param p⇠a⦄ ~~> b
                             ->               CALL p ON g // e ~~> b
 
   where "f // e ~~> v" := (fun_sem f e v). 
@@ -93,7 +90,7 @@ Section fun_sem.
                    | f u x y v e a H1 IH1 H2 IH2 
                    | f u x y v e a b c H1 IH1 H2 IH2 
                    | x f g e a b H1 IH1 H2 IH2 
-                   | p x f g e a b H1 H2 IH2 H3 IH3 ].
+                   | p g e a b H1 IH1 H2 IH2 ].
     + inversion 1; auto.
     + inversion 1; auto.
     + inversion 1; f_equal; auto.
@@ -106,67 +103,8 @@ Section fun_sem.
     + inversion 1.
       apply IH1 in H7; subst; auto.
     + inversion 1.
-      rewrite H1 in H5; inversion H5; subst.
-      apply IH2 in H6; subst; auto.
+      apply IH1 in H4; subst.
+      apply IH2 in H7; subst; auto.
   Qed.
 
 End fun_sem.
-
-Section mirror.
-
-  Variables (u x y z : Var) (Hxy : x <> y).
-  Variable (p : Fun).
-
-  Definition fe_mirror := MATCH £u WITH ø⇒ø OR x#y⇒CALL p ON £y#CALL p ON £x.
-
-  Variable (P : fun_prog) (HP : P⇢p = (u,fe_mirror)).
-
-  Local Notation "f // e ~~> v" := (fun_sem P f e v).
-
-  Fact fe_mirror_spec_1 f e a b : f // e ~~> a -> a ⋈ b -> CALL p ON f // e ~~> b.
-  Proof.
-    intros H1 H2; revert H2 f e H1.
-    induction 1 as [ | a b c d H1 IH1 H2 IH2 ]; intros f e H3.
-    + constructor 7 with u fe_mirror ω; auto.
-      unfold fe_mirror.
-      constructor 4.
-      * apply fs_var; rew env.
-      * constructor.
-    + constructor 7 with u fe_mirror ⟨a,c⟩; auto.
-      unfold fe_mirror.
-      constructor 5 with a c.
-      * apply fs_var; rew env.
-      * constructor 3.
-        - apply IH2, fs_var; rew env.
-        - apply IH1, fs_var; rew env.
-  Qed.
-
-  Fact fe_mirror_halt f e a : f // e ~~> a -> exists b, CALL p ON f // e ~~> b.
-  Proof.
-    intros H.
-    destruct (bt_compute_mirror a) as (b & Hb).
-    exists b; apply fe_mirror_spec_1 with (1 := H); auto.
-  Qed.
-
-  Fact fe_mirror_spec_2 f e a b : f // e ~~> a -> CALL p ON f // e ~~> b -> a ⋈ b.
-  Proof.
-    intros H1 H2.
-    destruct (bt_compute_mirror a) as (b' & Hb').
-    generalize (fe_mirror_spec_1 H1 Hb'); intros H3.
-    rewrite (fun_sem_det H2 H3); trivial.
-  Qed.
-
-  Theorem fe_mirror_spec e : exists m, CALL p ON £z // e ~~> m /\ e⇢z ⋈ m.
-  Proof.
-    destruct fe_mirror_halt with (£z) e (e⇢z) as (m & Hm).
-    + constructor 1.
-    + exists m; split; auto.
-      revert Hm; apply fe_mirror_spec_2.
-      constructor 1.
-  Qed.
-
-End mirror.
-
-Local Notation "f / P / e ~~> v" := (fun_sem P f e v) (at level 70, format "f  / P /  e  ~~>  v", no associativity).
-
-Check fe_mirror_spec.
