arith.v
@@ -1,0 +1,120 @@
+(**************************************************************)
+(*   Copyright Dominique Larchey-Wendling [*]                 *)
+(*                                                            *)
+(*                             [*] Affiliation LORIA -- CNRS  *)
+(**************************************************************)
+(*      This file is distributed under the terms of the       *)
+(*         CeCILL v2 FREE SOFTWARE LICENSE AGREEMENT          *)
+(**************************************************************)
+
+Require Import List Arith Lia Wellfounded.
+
+Require Import bt env fun_defs.
+
+Set Implicit Arguments.
+
+Local Notation "e ⇢ x" := (@get_env _ _ e x).
+Local Notation "e ⦃  x ⇠ v ⦄" := (@set_env _ _ Var_eq_dec e x v).
+
+Section arith.
+
+  Variables (u x y z : Var) (Hxy : x <> y) (Hxz : x <> z) (Hyz : y <> z).
+
+  Variable (p_add p_mul p_size : Fun).
+
+  Definition fe_add := 
+    MATCH £u WITH
+         ø   ⇒ ø 
+      OR x#z ⇒ 
+      MATCH £x WITH
+           ø   ⇒ £z 
+        OR x#y ⇒ ø#CALL p_add ON (£y#£z).
+
+  Definition fe_mul :=
+    MATCH £u WITH
+         ø   ⇒ ø 
+      OR x#z ⇒ 
+      MATCH £x WITH
+           ø   ⇒ ø
+        OR x#y ⇒ CALL p_add ON (£z#CALL p_mul ON (£y#£z)).
+
+  Definition fe_size :=
+    MATCH £u WITH
+         ø   ⇒ ø#ø
+      OR x#y ⇒ ø#CALL p_add ON (CALL p_size ON £x#CALL p_size ON £y).
+
+  Variable (param : Fun -> Var)     
+           (body : Fun -> fun_expr) 
+           
+           (Hparam_add : param p_add = u)    
+           (Hparam_mul : param p_mul = u)
+           (Hparam_size : param p_size = u) 
+
+           (Hbody_add : body p_add = fe_add) 
+           (Hbody_mul : body p_mul = fe_mul)
+           (Hbody_size : body p_size = fe_size).
+
+  Notation "f // s ~~> v" := (fun_sem param body f s v).
+
+  Fact fe_add_spec f e a b : f // e ~~> ⟨a,b⟩ -> CALL p_add ON f // e ~~> bt_add a b.
+  Proof.
+    revert f e; induction a as [ | a1 IH1 a2 IH2 ]; intros f e H3; simpl; 
+      constructor 7 with (1 := H3); rewrite Hbody_add, Hparam_add; unfold fe_add.
+    + constructor 5 with ω b.
+      1: apply fs_var; rew env.
+      constructor 4; apply fs_var; rew env.
+    + constructor 5 with ⟨a1,a2⟩ b.
+      1: apply fs_var; rew env.
+      constructor 5 with a1 a2.
+      1: apply fs_var; rew env.
+      constructor 3.
+      1: constructor 2.
+      apply IH2.
+      constructor 3; apply fs_var; rew env.
+  Qed.
+
+  Fact fe_mul_spec f e a b : f // e ~~> ⟨a,b⟩ -> CALL p_mul ON f // e ~~> bt_mul a b.
+  Proof.
+    revert f e; induction a as [ | a1 IH1 a2 IH2 ]; intros f e H3; simpl; 
+      constructor 7 with (1 := H3); rewrite Hbody_mul, Hparam_mul; unfold fe_mul.
+    + constructor 5 with ω b.
+      1: apply fs_var; rew env.
+      constructor 4. 
+      * apply fs_var; rew env.
+      * constructor 2.
+    + constructor 5 with ⟨a1,a2⟩ b.
+      1: apply fs_var; rew env.
+      constructor 5 with a1 a2.
+      1: apply fs_var; rew env.
+      apply fe_add_spec.
+      constructor 3.
+      1: apply fs_var; rew env.
+      apply IH2.
+      constructor 3; apply fs_var; rew env.
+  Qed.
+
+  Fact fe_size_spec f e t : f // e ~~> t -> CALL p_size ON f // e ~~> bt_size t.
+  Proof.
+    revert f e; induction t as [ | a IHa b IHb ]; intros f e H; simpl;
+      constructor 7 with (1 := H); rewrite Hbody_size, Hparam_size; unfold fe_size.
+    + constructor 4.
+      1: apply fs_var; rew env.
+      constructor 3; constructor 2.
+    + constructor 5 with a b.
+      1: apply fs_var; rew env.
+      constructor 3.
+      1: constructor 2.
+      apply fe_add_spec.
+      constructor 3.
+      * apply IHa, fs_var; rew env.
+      * apply IHb, fs_var; rew env.
+  Qed.
+
+End arith.
+
+Local Notation "f // e ~~> v [ p , b ]" := (fun_sem p b f e v) (at level 70, format "f  //  e  ~~>  v  [ p , b ]", no associativity).
+
+Check fe_add_spec.
+Check fe_mul_spec.
+Check fe_size_spec.
+
