mirror.v
@@ -1,0 +1,70 @@
+(**************************************************************)
+(*   Copyright Dominique Larchey-Wendling [*]                 *)
+(*                                                            *)
+(*                             [*] Affiliation LORIA -- CNRS  *)
+(**************************************************************)
+(*      This file is distributed under the terms of the       *)
+(*         CeCILL v2 FREE SOFTWARE LICENSE AGREEMENT          *)
+(**************************************************************)
+
+Require Import List Arith Lia Wellfounded.
+
+Require Import bt env fun_defs.
+
+Set Implicit Arguments.
+
+Local Notation "e ⇢ x" := (@get_env _ _ e x).
+Local Notation "e ⦃  x ⇠ v ⦄" := (@set_env _ _ Var_eq_dec e x v).
+
+Section mirror.
+
+  Variables (u x y z : Var) (Hxy : x <> y).
+  Variable (p : Fun).
+
+  Definition fe_mirror := MATCH £u WITH ø⇒ø OR x#y⇒CALL p ON £y#CALL p ON £x.
+
+  Variable (param : Fun -> Var)     (Hparam : param p = u) 
+           (body : Fun -> fun_expr) (Hbody : body p = fe_mirror).
+
+  Notation "f // s ~~> v" := (fun_sem param body f s v).
+
+  Fact fe_mirror_spec_1 f e a b : f // e ~~> a -> a ⋈ b -> CALL p ON f // e ~~> b.
+  Proof.
+    intros H1 H2; revert H2 f e H1.
+    induction 1 as [ | a b c d H1 IH1 H2 IH2 ]; intros f e H3;
+      constructor 7 with (1 := H3);
+      rewrite Hparam, Hbody; unfold fe_mirror.
+    + constructor 4.
+      * apply fs_var; rew env.
+      * constructor.
+    + constructor 5 with a c.
+      * apply fs_var; rew env.
+      * constructor 3.
+        - apply IH2, fs_var; rew env.
+        - apply IH1, fs_var; rew env.
+  Qed.
+
+  Hint Resolve btm_spec.
+
+  Fact fe_mirror_halt f e a : f // e ~~> a -> CALL p ON f // e ~~> btm a.
+  Proof.
+    intros H; apply fe_mirror_spec_1 with (1 := H); auto.
+  Qed.
+
+  Fact fe_mirror_spec_2 f e a b : f // e ~~> a -> CALL p ON f // e ~~> b <-> a ⋈ b.
+  Proof.
+    intros H1; split.
+    + intros H2.
+      rewrite (fun_sem_det H2 (fe_mirror_halt H1)); auto.
+    + apply fe_mirror_spec_1; auto.
+  Qed.
+
+  Theorem fe_mirror_spec e : CALL p ON £z // e ~~> btm (e⇢z).
+  Proof. apply fe_mirror_halt; constructor. Qed.
+
+End mirror.
+
+Local Notation "f // e ~~> v [ p , b ]" := (fun_sem p b f e v) (at level 70, format "f  //  e  ~~>  v  [ p , b ]", no associativity).
+
+Check fe_mirror_spec.
+
